.

theories/Data/Graph.v
@@ -145,7 +145,7 @@ Lemma mk_subpath (v0 : V) (v1 : V) (v : V) (p : list V)
 Proof.
   revert v1 ELEM. induction PATH as [ | v0 v1 p H_edge PATH IH NOT_IN]; i; inv ELEM.
   - exists [v2]. split; eauto.
-  - rename H into ELEM. pose proof (IH v2 ELEM) as (p'&PATH1&p''&PATH2&EQ).
+  - obtain (p'&PATH1&p''&PATH2&EQ) by IH.
     exists (v1 :: p'). split.
     + econstructor 2; eauto. subst p. rewrite in_app_iff in NOT_IN. tauto.
     + exists p''. split; [exact PATH2 | now rewrite EQ].
@@ -162,8 +162,7 @@ Proof.
   - rewrite -> walk_app_iff in WALK. destruct WALK as (v1&WALK1&WALK2).
     inv WALK2. inv H_walk. pose proof (IH v0 v1 WALK1) as [p PATH].
     pose proof (In_dec v' p) as [ELEM | NOT_IN].
-    + pose proof (mk_subpath v0 v' v1 p PATH ELEM) as (p'&PATH'&_).
-      exists p'. exact PATH'.
+    + obtain (p'&PATH'&_) by (mk_subpath _ _ _ _ PATH). ss!.
     + exists (p ++ [v']). rewrite -> path_iff_no_dup_walk. split.
       * rewrite -> walk_app_iff. exists v1. split.
         { now eapply path_iff_no_dup_walk. }
@@ -339,7 +338,7 @@ Proof.
     + rewrite -> L.existsb_exists in REACH.
       destruct REACH as (z & z_in & REACH).
       destruct (E_dec x z) as [EDGE | NO_EDGE]; try discriminate.
-      pose proof (IH z y REACH) as (w & LENGTH & WALK).
+      find (w & LENGTH & WALK) by (IH z y).
       exists (z :: w). split; [simpl; lia | econstructor 2; eauto].
 Qed.
 
@@ -381,8 +380,8 @@ Lemma reachableb_iff_reachable (x : V) (y : V)
   : reachableb (L.length vertices') x y = true <-> y \in reachable x.
 Proof.
   split.
-  - intros REACH.
-    pose proof (reachableb_elim _ _ _ REACH) as (w & _ & WALK).
+  - i.
+    find (w & _ & WALK) by (reachableb_elim (length vertices') x y).
     now exists w.
   - intros [w WALK].
     assert (exists p, x ---[ p ]-->*( G ) y) as [p PATH].
@@ -432,7 +431,7 @@ Lemma reachable_step (x : V) (y : V) (z : V)
   (REACH : z \in reachable y)
   : z \in reachable x.
 Proof.
-  destruct REACH as [w WALK]. exists (y :: w). econstructor; eauto.
+  destruct REACH as [w WALK]. exists (y :: w). econs 2; eauto.
 Qed.
 
 Lemma gmu_reachable_seed (x : V) (a : A)
@@ -440,8 +439,8 @@ Lemma gmu_reachable_seed (x : V) (a : A)
   : exists y, y \in reachable x /\ a \in seed y.
 Proof.
   induction IN as [x a SEED | x y EDGE a IN (z & REACH & SEED)].
-  - exists x. split; [exists []; econstructor 1 | exact SEED].
-  - exists z. split; [eapply reachable_step; eauto | exact SEED].
+  - exists x. split; [exists []; econs 1 | auto].
+  - exists z. split; [eapply reachable_step; eauto | auto].
 Qed.
 
 Lemma gmu_iff_reachable_seed (x : V) (a : A)
@@ -458,8 +457,8 @@ Definition gmu' (x : V) : fin_ensemble A :=
 Theorem gmu_sim (x : V)
   : gmu' x =~= gmu x.
 Proof.
-  pose proof (list_corresponds_to_finite_ensemble_flat_map (reachable' x) (reachable x) seed' seed (reachable_sim x) (fun x : V => fun _ => seed_sim x)) as FLAT_MAP.
-  rewrite list_corresponds_to_finite_ensemble_iff in FLAT_MAP |- *. intros a. rewrite FLAT_MAP. symmetry. eapply gmu_iff_reachable_seed.
+  find H by (list_corresponds_to_finite_ensemble_flat_map (reachable' x) (reachable x) _ _ (reachable_sim x)).
+  rewrite list_corresponds_to_finite_ensemble_iff in H |- *. i. rewrite H. symmetry. eapply gmu_iff_reachable_seed.
 Qed.
 
 End DIGRAPH_FIXEDPOINT.
@@ -477,13 +476,7 @@ Section DIGRAPH.
 #[local] Infix "\in" := E.In.
 #[local] Infix "∈" := L.In.
 
-Context {X : Type}.
-
-Fixpoint digraph_value {A : Type} `{EQ_DEC : hasEqDec A} (fuel : nat) (seed : X -> fin_ensemble A) (deps : X -> fin_ensemble X) (x : X) : fin_ensemble A :=
-  match fuel with
-  | O => normalize (seed x)
-  | S fuel' => normalize (union (seed x) (flat_map (digraph_value fuel' seed deps) (deps x)))
-  end.
+Context {X : Type} {A : Type}.
 
 Inductive digraph_closure {A : Type} (seed : X -> fin_ensemble A) (deps : X -> fin_ensemble X) (a : A) (x : X) : Prop :=
   | digraph_closure_seed
@@ -503,7 +496,7 @@ Inductive digraph_trace {A : Type} (seed : X -> fin_ensemble A) (deps : X -> fin
     (TRACE : digraph_trace seed deps a y tr)
     : y :: tr \in digraph_trace seed deps a x.
 
-Theorem digraph_closure_iff_trace {A : Type} (seed : X -> fin_ensemble A) (deps : X -> fin_ensemble X) (x : X) (a : A)
+Theorem digraph_closure_iff_trace (seed : X -> fin_ensemble A) (deps : X -> fin_ensemble X) (x : X) (a : A)
   : digraph_closure seed deps a x <-> (exists tr, tr \in digraph_trace seed deps a x).
 Proof.
   split.
@@ -515,7 +508,7 @@ Proof.
     + eapply digraph_closure_step; eauto.
 Qed.
 
-Lemma digraph_trace_in_nodes {A : Type} (nodes : fin_ensemble X) (seed : X -> fin_ensemble A) (deps : X -> fin_ensemble X) (x : X) (a : A) (tr : list X)
+Lemma digraph_trace_in_nodes (nodes : fin_ensemble X) (seed : X -> fin_ensemble A) (deps : X -> fin_ensemble X) (x : X) (a : A) (tr : list X)
   (deps_CLOSED : forall x, forall y, y ∈ deps x -> y ∈ nodes)
   (TRACE : tr \in digraph_trace seed deps a x)
   : Forall (fun y => y ∈ nodes) tr.
@@ -529,21 +522,21 @@ Definition digraph_graph (deps : X -> fin_ensemble X) : GRAPH.t :=
     GRAPH.edges := fun '(x, x') => x' ∈ deps x;
   |}.
 
-Lemma digraph_trace_seed_at_last {A : Type} (seed : X -> fin_ensemble A) (deps : X -> fin_ensemble X) (x : X) (a : A) (tr : list X)
+Lemma digraph_trace_seed_at_last (seed : X -> fin_ensemble A) (deps : X -> fin_ensemble X) (x : X) (a : A) (tr : list X)
   (TRACE : tr \in digraph_trace seed deps a x)
   : a ∈ seed (last tr x).
 Proof.
   induction TRACE as [x IN | x y tr EDGE TRACE IH]; ss!.
 Qed.
 
-Lemma digraph_trace_walk {A : Type} (seed : X -> fin_ensemble A) (deps : X -> fin_ensemble X) (x : X) (a : A) (tr : list X)
+Lemma digraph_trace_walk (seed : X -> fin_ensemble A) (deps : X -> fin_ensemble X) (x : X) (a : A) (tr : list X)
   (TRACE : tr \in digraph_trace seed deps a x)
   : x ~~~[ tr ]~~>*( digraph_graph deps ) last tr x.
 Proof.
   induction TRACE as [x IN | x y tr EDGE TRACE IH]; ss!.
 Qed.
 
-Lemma digraph_walk_trace {A : Type} (seed : X -> fin_ensemble A) (deps : X -> fin_ensemble X) (x : X) (a : A) (x' : X) (tr : list X)
+Lemma digraph_walk_trace (seed : X -> fin_ensemble A) (deps : X -> fin_ensemble X) (x : X) (a : A) (x' : X) (tr : list X)
   (WALK : x ~~~[ tr ]~~>*( digraph_graph deps ) x')
   (IN : a ∈ seed x')
   : tr \in digraph_trace seed deps a x.
@@ -551,21 +544,21 @@ Proof.
   induction WALK as [ | v0 v1 w EDGE WALK IH]; now constructor.
 Qed.
 
-Lemma digraph_trace_simple {A : Type} `{X_hasEqDec : hasEqDec X} (seed : X -> fin_ensemble A) (deps : X -> fin_ensemble X) (x : X) (a : A) (tr : list X)
+Lemma digraph_trace_simple `{X_hasEqDec : hasEqDec X} (seed : X -> fin_ensemble A) (deps : X -> fin_ensemble X) (x : X) (a : A) (tr : list X)
   (TRACE : tr \in digraph_trace seed deps a x)
   : exists simple, digraph_trace seed deps a x simple /\ NoDup simple.
 Proof.
   pose proof (digraph_trace_walk seed deps x a tr TRACE) as WALK.
   pose proof (digraph_trace_seed_at_last seed deps x a tr TRACE) as SEED.
-  assert (exists simple, x ---[ simple ]-->*( digraph_graph deps ) last tr x) as [simple PATH].
+  assert (exists simple : list GRAPH.vertices, x ---[ simple ]-->*( digraph_graph deps ) last tr x) as [simple PATH].
   { eapply walk_finds_path with (w := tr); auto. intros v vs.
     now pose proof (@L.in_dec X X_hasEqDec v vs) as [YES | NO]; [left | right].
   }
   rewrite path_iff_no_dup_walk in PATH. destruct PATH as [WALK' NO_DUP].
-  exists simple; split; [eapply digraph_walk_trace; eauto | exact NO_DUP].
+  obtain ? by (digraph_walk_trace seed deps _ _ _ simple). ss!.
 Qed.
 
-Lemma digraph_trace_simple_bounded {A : Type} `{X_hasEqDec : hasEqDec X} (nodes : fin_ensemble X) (seed : X -> fin_ensemble A) (deps : X -> fin_ensemble X) (x : X) (a : A) (tr : list X)
+Lemma digraph_trace_simple_bounded `{X_hasEqDec : hasEqDec X} (nodes : fin_ensemble X) (seed : X -> fin_ensemble A) (deps : X -> fin_ensemble X) (x : X) (a : A) (tr : list X)
   (deps_CLOSED : forall x, forall y, y ∈ deps x -> y ∈ nodes)
   (TRACE : tr \in digraph_trace seed deps a x)
   : exists simple, simple \in digraph_trace seed deps a x /\ length simple <= length nodes.
@@ -576,17 +569,49 @@ Proof.
   rewrite Forall_forall in IN_NODES. now eapply IN_NODES.
 Qed.
 
-Definition digraph_equation {A : Type} (seed : X -> fin_ensemble A) (deps : X -> fin_ensemble X) (value : X -> fin_ensemble A) : Prop :=
+Definition digraph_equation (seed : X -> fin_ensemble A) (deps : X -> fin_ensemble X) (value : X -> fin_ensemble A) : Prop :=
   forall x, forall a, a ∈ value x <-> ⟪ UNFOLD : a ∈ seed x \/ (exists y, y ∈ deps x /\ a ∈ value y) ⟫.
 
-Lemma digraph_value_seed {A : Type} `{EQ_DEC : hasEqDec A} (fuel : nat) (seed : X -> fin_ensemble A) (deps : X -> fin_ensemble X) (x : X) (a : A)
+#[local] Open Scope function_scope.
+
+Definition digraph_fixedpoint (seed : X -> fin_ensemble A) (deps : X -> fin_ensemble X) (value' : X -> ensemble A) : Prop :=
+  forall x, forall a, a \in value' x <-> ⟪ STEP : a ∈ seed x \/ (exists y, y ∈ deps x /\ a \in value' y) ⟫.
+
+Theorem digraph_closure_fixedpoint (seed : X -> fin_ensemble A) (deps : X -> fin_ensemble X)
+  : digraph_fixedpoint seed deps (fun x => { a : A | digraph_closure seed deps a x }).
+Proof.
+  intros x a. unfold E.In; unnw. split.
+  - intros CLOSURE. destruct CLOSURE as [SEED_IN | y EDGE CLOSURE].
+    + now left.
+    + now right; exists y.
+  - intros [SEED_IN | (y & EDGE & CLOSURE)].
+    + now eapply digraph_closure_seed.
+    + now eapply digraph_closure_step with (y := y).
+Qed.
+
+Theorem digraph_closure_least_fixedpoint (seed : X -> fin_ensemble A) (deps : X -> fin_ensemble X) (value : X -> ensemble A)
+  (FIXPOINT : digraph_fixedpoint seed deps value)
+  : forall x, { a : A | digraph_closure seed deps a x } \subseteq value x.
+Proof.
+  intros x a CLOSURE; induction CLOSURE as [x SEED_IN | x y EDGE CLOSURE IH]; ss!.
+Qed.
+
+Context `{EQ_DEC : hasEqDec A}.
+
+Fixpoint digraph_value (fuel : nat) (seed : X -> fin_ensemble A) (deps : X -> fin_ensemble X) (x : X) : fin_ensemble A :=
+  match fuel with
+  | O => normalize (seed x)
+  | S fuel' => normalize (union (seed x) (flat_map (digraph_value fuel' seed deps) (deps x)))
+  end.
+
+Lemma digraph_value_seed (fuel : nat) (seed : X -> fin_ensemble A) (deps : X -> fin_ensemble X) (x : X) (a : A)
   (IN : a ∈ seed x)
   : a ∈ digraph_value fuel seed deps x.
 Proof.
   destruct fuel as [ | fuel]; ss!.
 Qed.
 
-Lemma digraph_value_propagated {A : Type} `{EQ_DEC : hasEqDec A} (fuel : nat) (seed : X -> fin_ensemble A) (deps : X -> fin_ensemble X) (x : X) (y : X) (a : A)
+Lemma digraph_value_propagated (fuel : nat) (seed : X -> fin_ensemble A) (deps : X -> fin_ensemble X) (x : X) (y : X) (a : A)
   (EDGE : y ∈ deps x)
   (IN : a ∈ digraph_value fuel seed deps y)
   : a ∈ digraph_value (S fuel) seed deps x.
@@ -594,7 +619,7 @@ Proof.
   ss!.
 Qed.
 
-Theorem digraph_value_elim {A : Type} `{EQ_DEC : hasEqDec A} (fuel : nat) (seed : X -> fin_ensemble A) (deps : X -> fin_ensemble X) (x : X) (a : A)
+Theorem digraph_value_elim (fuel : nat) (seed : X -> fin_ensemble A) (deps : X -> fin_ensemble X) (x : X) (a : A)
   (IN : a ∈ digraph_value fuel seed deps x)
   : digraph_closure seed deps a x.
 Proof.
@@ -605,14 +630,14 @@ Proof.
     + eapply digraph_closure_step; ss!.
 Qed.
 
-Lemma digraph_value_monotone_step {A : Type} `{EQ_DEC : hasEqDec A} (fuel : nat) (seed : X -> fin_ensemble A) (deps : X -> fin_ensemble X) (x : X) (a : A)
+Lemma digraph_value_monotone_step (fuel : nat) (seed : X -> fin_ensemble A) (deps : X -> fin_ensemble X) (x : X) (a : A)
   (IN : a ∈ digraph_value fuel seed deps x)
   : a ∈ digraph_value (S fuel) seed deps x.
 Proof.
   revert x a IN; induction fuel as [ | fuel IH]; intros x a IN; simpl in IN |- *; ss!.
 Qed.
 
-Lemma digraph_value_monotone {A : Type} `{EQ_DEC : hasEqDec A} (fuel1 : nat) (fuel2 : nat) (seed : X -> fin_ensemble A) (deps : X -> fin_ensemble X) (x : X) (a : A)
+Lemma digraph_value_monotone (fuel1 : nat) (fuel2 : nat) (seed : X -> fin_ensemble A) (deps : X -> fin_ensemble X) (x : X) (a : A)
   (LE : fuel1 <= fuel2)
   (IN : a ∈ digraph_value fuel1 seed deps x)
   : a ∈ digraph_value fuel2 seed deps x.
@@ -625,7 +650,7 @@ Proof.
     + eapply digraph_value_monotone_step. eapply IH with (fuel1 := fuel1) (x := x) (a := a); done!.
 Qed.
 
-Theorem digraph_trace_value {A : Type} `{EQ_DEC : hasEqDec A} (seed : X -> fin_ensemble A) (deps : X -> fin_ensemble X) (x : X) (a : A) (tr : list X) (fuel : nat)
+Theorem digraph_trace_value (seed : X -> fin_ensemble A) (deps : X -> fin_ensemble X) (x : X) (a : A) (tr : list X) (fuel : nat)
   (TRACE : tr \in digraph_trace seed deps a x)
   (LE : length tr <= fuel)
   : a ∈ digraph_value fuel seed deps x.
@@ -635,7 +660,7 @@ Proof.
   - destruct fuel as [ | fuel]; simpl in LE; [lia | eapply digraph_value_propagated]; done!.
 Qed.
 
-Theorem digraph_closure_intro {A : Type} `{EQ_DEC : hasEqDec A} (seed : X -> fin_ensemble A) (deps : X -> fin_ensemble X) (x : X) (a : A)
+Theorem digraph_closure_intro (seed : X -> fin_ensemble A) (deps : X -> fin_ensemble X) (x : X) (a : A)
   (IN : digraph_closure seed deps a x)
   : exists fuel, a ∈ digraph_value fuel seed deps x.
 Proof.
@@ -644,7 +669,7 @@ Proof.
   - destruct IH as [fuel VALUE_IN]. exists (S fuel). eapply digraph_value_propagated; eauto.
 Qed.
 
-Theorem digraph_closure_least {A : Type} (seed : X -> fin_ensemble A) (deps : X -> fin_ensemble X) (value : X -> fin_ensemble A) (x : X) (a : A)
+Theorem digraph_closure_least (seed : X -> fin_ensemble A) (deps : X -> fin_ensemble X) (value : X -> fin_ensemble A) (x : X) (a : A)
   (EQUATION : digraph_equation seed deps value)
   (IN : digraph_closure seed deps a x)
   : a ∈ value x.
@@ -654,42 +679,20 @@ Proof.
   - exact (proj2 (EQUATION x a) (or_intror (@ex_intro _ _ y (conj EDGE IH)))).
 Qed.
 
-#[local] Open Scope function_scope.
+Context `{X_hasEqDec : hasEqDec X}.
 
-Definition digraph_fixedpoint {A : Type} (seed : X -> fin_ensemble A) (deps : X -> fin_ensemble X) (value' : X -> ensemble A) : Prop :=
-  forall x, forall a, a \in value' x <-> ⟪ STEP : a ∈ seed x \/ (exists y, y ∈ deps x /\ a \in value' y) ⟫.
-
-Theorem digraph_closure_fixedpoint {A : Type} (seed : X -> fin_ensemble A) (deps : X -> fin_ensemble X)
-  : digraph_fixedpoint seed deps (fun x => { a : A | digraph_closure seed deps a x }).
-Proof.
-  intros x a. unfold E.In; unnw. split.
-  - intros CLOSURE. destruct CLOSURE as [SEED_IN | y EDGE CLOSURE].
-    + now left.
-    + now right; exists y.
-  - intros [SEED_IN | (y & EDGE & CLOSURE)].
-    + now eapply digraph_closure_seed.
-    + now eapply digraph_closure_step with (y := y).
-Qed.
-
-Theorem digraph_closure_least_fixedpoint {A : Type} (seed : X -> fin_ensemble A) (deps : X -> fin_ensemble X) (value : X -> ensemble A)
-  (FIXPOINT : digraph_fixedpoint seed deps value)
-  : forall x, { a : A | digraph_closure seed deps a x } \subseteq value x.
-Proof.
-  intros x a CLOSURE; induction CLOSURE as [x SEED_IN | x y EDGE CLOSURE IH]; ss!.
-Qed.
-
-Theorem digraph_closure_intro_bounded {A : Type} `{EQ_DEC : hasEqDec A} `{X_hasEqDec : hasEqDec X} (fuel : nat) (nodes : fin_ensemble X) (seed : X -> fin_ensemble A) (deps : X -> fin_ensemble X) (x : X) (a : A)
+Theorem digraph_closure_intro_bounded (fuel : nat) (nodes : fin_ensemble X) (seed : X -> fin_ensemble A) (deps : X -> fin_ensemble X) (x : X) (a : A)
   (fuel_ENOUGH : length nodes <= fuel)
   (deps_CLOSED : forall x, forall y, y ∈ deps x -> y ∈ nodes)
   (IN : digraph_closure seed deps a x)
   : a ∈ digraph_value fuel seed deps x.
 Proof.
   rewrite digraph_closure_iff_trace in IN. destruct IN as [tr TRACE].
-  pose proof (digraph_trace_simple_bounded nodes seed deps x a tr deps_CLOSED TRACE) as (simple & TRACE' & LENGTH).
+  find (simple & TRACE' & LENGTH) by (digraph_trace_simple_bounded nodes seed deps).
   eapply digraph_trace_value with (tr := simple); ss!.
 Qed.
 
-Theorem digraph_value_iff_closure_bounded {A : Type} `{EQ_DEC : hasEqDec A} `{X_hasEqDec : hasEqDec X} (fuel : nat) (nodes : fin_ensemble X) (seed : X -> fin_ensemble A) (deps : X -> fin_ensemble X) (x : X) (a : A)
+Theorem digraph_value_iff_closure_bounded (fuel : nat) (nodes : fin_ensemble X) (seed : X -> fin_ensemble A) (deps : X -> fin_ensemble X) (x : X) (a : A)
   (fuel_ENOUGH : length nodes <= fuel)
   (deps_CLOSED : forall x, forall y, y ∈ deps x -> y ∈ nodes)
   : a ∈ digraph_value fuel seed deps x <-> digraph_closure seed deps a x.
@@ -702,517 +705,3 @@ Qed.
 End DIGRAPH.
 
 End DigraphFixedpoint.
-
-#[local] Hint Rewrite L.in_remove_iff : simplication_hints.
-
-Module GraphAPI.
-
-#[local] Infix "=~=" := is_similar_to.
-
-#[universes(template), projections(primitive)]
-Class FiniteGraph `{V : Type} : Type :=
-  mkFiniteGraph
-  { E : ensemble (V * V)
-  ; G := {| GRAPH.vertices := V; GRAPH.edges := E |}
-  ; V_dec : hasEqDec V
-  ; E_dec (v : V) (v' : V) : B.Decision ((v, v') \in E) 
-  ; enum_vertices : fin_ensemble V
-  ; enum_vertices_contains_all
-    : exists extras : ensemble V, enum_vertices =~= E.union { v : V | (exists v_in, (v_in, v) \in E) \/ (exists v_out, (v, v_out) \in E) } extras
-  } as GRAPH.
-
-#[global] Arguments E {V} GRAPH.
-#[global] Arguments enum_vertices_contains_all {V} GRAPH : simpl never.
-
-#[local] Existing Instance G.
-#[global] Existing Instance V_dec.
-#[global] Existing Instance E_dec.
-
-Notation " src '~~~[' w ']~~>*('  GRAPH  ')' tgt " := (@walk GRAPH.(G) tgt src w).
-Notation " src '---[' p ']-->*('  GRAPH  ')' tgt " := (@path GRAPH.(G) tgt src p).
-Notation " src '===[' t ']==>*('  GRAPH  ')' tgt " := (@trail GRAPH.(G) tgt src t).
-
-Abbreviation gmu := (DigraphFixedpoint.gmu (G := G)).
-
-Section FiniteGraph_CONSTRUCTION.
-
-#[local] Obligation Tactic := i.
-
-Context {V : Type}.
-
-#[refine]
-Definition emptyFiniteGraph `{V_hasEqDec : hasEqDec V} : @FiniteGraph V :=
-  {|
-    E := fun '(v, v') => False;
-    V_dec := V_hasEqDec;
-    E_dec := fun v : V => fun v' : V => B.decide _;
-    enum_vertices := [];
-  |}.
-Proof.
-  rewrite FS.subset_lemma in *. done.
-Defined.
-
-Lemma emptyFiniteGraph_edge_spec {V_hasEqDec : hasEqDec V}
-  : forall edge : V * V, edge \in (emptyFiniteGraph).(E) <-> edge \in E.empty.
-Proof.
-  intros [v v']; done.
-Qed.
-
-#[refine]
-Definition insertEdge (v_in : V) (v_out : V) (GRAPH : @FiniteGraph V) : @FiniteGraph V :=
-  {|
-    E := fun '(v, v') => (v = v_in /\ v' = v_out) \/ E.In (v, v') GRAPH.(E);
-    V_dec := GRAPH.(V_dec);
-    E_dec := fun v : V => fun v' : V => B.decide _;
-    enum_vertices := v_in :: v_out :: GRAPH.(enum_vertices);
-  |}.
-Proof.
-  pose proof GRAPH.(enum_vertices_contains_all) as HH.
-  rewrite FS.subset_lemma in *. done.
-Defined.
-
-Lemma insertEdge_edge_spec v_in v_out GRAPH
-  : forall edge : V * V, edge \in (insertEdge v_in v_out GRAPH).(E) <-> edge \in E.insert (v_in, v_out) GRAPH.(E).
-Proof.
-  intros [v v']; done.
-Qed.
-
-#[refine]
-Definition removeEdge (v_in : V) (v_out : V) (GRAPH : @FiniteGraph V) : @FiniteGraph V :=
-  {|
-    E := fun '(v, v') => (~ (v = v_in /\ v' = v_out)) /\ E.In (v, v') GRAPH.(E);
-    V_dec := GRAPH.(V_dec);
-    E_dec := fun v : V => fun v' : V => B.decide _;
-    enum_vertices := GRAPH.(enum_vertices);
-  |}.
-Proof.
-  pose proof GRAPH.(enum_vertices_contains_all) as HH.
-  rewrite FS.subset_lemma in *. done.
-Defined.
-
-Lemma removeEdge_edge_spec v_in v_out GRAPH
-  : forall edge : V * V, edge \in (removeEdge v_in v_out GRAPH).(E) <-> edge \in E.delete (v_in, v_out) GRAPH.(E).
-Proof.
-  intros [v v']; done.
-Qed.
-
-#[refine]
-Definition insertVertex (v_new : V) (GRAPH : @FiniteGraph V) : @FiniteGraph V :=
-  {|
-    E := GRAPH.(E);
-    V_dec := GRAPH.(V_dec);
-    E_dec := GRAPH.(E_dec);
-    enum_vertices := v_new :: GRAPH.(enum_vertices);
-  |}.
-Proof.
-  pose proof GRAPH.(enum_vertices_contains_all) as HH.
-  rewrite FS.subset_lemma in *. done.
-Defined.
-
-Lemma insertVertex_edge_spec v_new GRAPH
-  : forall edge : V * V, edge \in (insertVertex v_new GRAPH).(E) <-> edge \in GRAPH.(E).
-Proof.
-  intros [v v']; done.
-Qed.
-
-#[refine]
-Definition removeVertex (v_old : V) (GRAPH : @FiniteGraph V) : @FiniteGraph V :=
-  {|
-    E := fun '(v, v') => v ≠ v_old /\ v' ≠ v_old /\ E.In (v, v') GRAPH.(E);
-    V_dec := GRAPH.(V_dec);
-    E_dec := fun v : V => fun v' : V => B.decide _;
-    enum_vertices := @L.remove V GRAPH.(V_dec) v_old GRAPH.(enum_vertices);
-  |}.
-Proof.
-  pose proof GRAPH.(enum_vertices_contains_all) as HH.
-  rewrite FS.subset_lemma in *. done.
-Defined.
-
-Lemma removeVertex_edge_spec v_old GRAPH
-  : forall edge : V * V, edge \in (removeVertex v_old GRAPH).(E) <-> (fst edge ≠ v_old /\ snd edge ≠ v_old /\ edge \in GRAPH.(E)).
-Proof.
-  intros [v v']; done.
-Qed.
-
-Class ColoredGraph {C : Type} (GRAPH : @FiniteGraph V) : Type :=
-  color_of_vertex : V -> C.
-
-End FiniteGraph_CONSTRUCTION.
-
-Section EXPORT.
-
-Context `{GRAPH : FiniteGraph}.
-
-#[local] Abbreviation E := GRAPH.(E).
-
-Lemma walk_last (v : V) (v' : V) (w : list V)
-  (WALK : v ~~~[ w ]~~>*( GRAPH ) v')
-  : v' = last w v.
-Proof.
-  exact (Graph.walk_last v v' w WALK).
-Qed.
-
-Theorem walk_iff (v : V) (w : list V)
-  : v ~~~[ w ]~~>*( GRAPH ) last w v <-> L.Forall E (L.mk_edge_seq v w).
-Proof.
-  exact (Graph.walk_iff v w).
-Qed.
-
-Lemma walk_app (v1 : V) (v2 : V) (v : V) (w1 : list V) (w2 : list V)
-  (WALK1 : v1 ~~~[ w1 ]~~>*( GRAPH ) v2)
-  (WALK2 : v2 ~~~[ w2 ]~~>*( GRAPH ) v)
-  : v1 ~~~[ w1 ++ w2 ]~~>*( GRAPH ) v.
-Proof.
-  exact (Graph.walk_app v1 v2 v w1 w2 WALK1 WALK2).
-Qed.
-
-Theorem walk_app_iff (v1 : V) (v : V) (w1 : list V) (w2 : list V)
-  : v1 ~~~[ w1 ++ w2 ]~~>*( GRAPH ) v <-> (exists v2, v1 ~~~[ w1 ]~~>*( GRAPH ) v2 /\ v2 ~~~[ w2 ]~~>*( GRAPH ) v).
-Proof.
-  exact (Graph.walk_app_iff v1 v w1 w2).
-Qed.
-
-Lemma path_vertices_no_dup (v : V) (v' : V) (p : list V)
-  (PATH : v ---[ p ]-->*( GRAPH ) v')
-  : NoDup p.
-Proof.
-  exact (Graph.path_vertices_no_dup v v' p PATH).
-Qed.
-
-Lemma no_dup_walk_is_path (v : V) (v' : V) (w : list V)
-  (NO_DUP : NoDup w)
-  (WALK : v ~~~[ w ]~~>*( GRAPH ) v')
-  : v ---[ w ]-->*( GRAPH ) v'.
-Proof.
-  exact (Graph.no_dup_walk_is_path v v' w NO_DUP WALK).
-Qed.
-
-Theorem path_iff_no_dup_walk (v : V) (v' : V) (w : list V)
-  : v ---[ w ]-->*( GRAPH ) v' <-> (v ~~~[ w ]~~>*( GRAPH ) v' /\ NoDup w).
-Proof.
-  exact (Graph.path_iff_no_dup_walk v v' w).
-Qed.
-
-Lemma path_app_inv (v1 : V) (v : V) (p1 : list V) (p2 : list V)
-  (PATH : v1 ---[ p1 ++ p2 ]-->*( GRAPH ) v)
-  : exists v2, v1 ---[ p1 ]-->*( GRAPH ) v2 /\ v2 ---[ p2 ]-->*( GRAPH ) v.
-Proof.
-  exact (Graph.path_app_inv v1 v p1 p2 PATH).
-Qed.
-
-Lemma mk_subpath (v0 : V) (v : V) (v' : V) (p : list V)
-  (PATH : v0 ---[ p ]-->*( GRAPH ) v')
-  (ELEM : In v p)
-  : exists p', v0 ---[ p' ]-->*( GRAPH ) v /\ (exists p'', v ---[ p'' ]-->*( GRAPH ) v' /\ p = p' ++ p'').
-Proof.
-  exact (Graph.mk_subpath v0 v v' p PATH ELEM).
-Qed.
-
-Theorem walk_finds_path (v : V) (v' : V) (w : list V)
-  (WALK : v ~~~[ w ]~~>*( GRAPH ) v')
-  : exists p, v ---[ p ]-->*( GRAPH ) v'.
-Proof.
-  eapply Graph.walk_finds_path with (w := w).
-  - ii. now pose proof (L.in_dec V_dec v0 vs) as [YES | NO]; [left | right].
-  - exact WALK.
-Qed.
-
-Lemma path_implies_trail (v : V) (v' : V) (p : list V)
-  (PATH : v ---[ p ]-->*( GRAPH ) v')
-  : v ===[ p ]==>*( GRAPH ) v'.
-Proof.
-  eapply Graph.path_implies_trail with (p := p). exact PATH.
-Qed.
-
-Definition reachable (v : V) : ensemble V :=
-  fun v' => exists w, v ~~~[ w ]~~>*( GRAPH ) v'.
-
-Lemma reachable_step (v : V) (v' : V) (v'' : V)
-  (EDGE : (v, v') \in E)
-  (REACHABLE : v'' \in reachable v')
-  : v'' \in reachable v.
-Proof.
-  exact (DigraphFixedpoint.reachable_step v v' v'' EDGE REACHABLE).
-Qed.
-
-Lemma enum_vertices_has_edge_tgt (v : V) (v' : V)
-  (EDGE : (v, v') \in E)
-  : L.In v' enum_vertices.
-Proof.
-  pose proof GRAPH.(enum_vertices_contains_all) as SIM. ss!.
-Qed.
-
-Fixpoint reachableb_accum (fuel : nat) (v : V) (v' : V) {struct fuel} : bool :=
-  match fuel with
-  | O => eqb v v'
-  | S fuel' => eqb v v' || L.existsb (fun v1 => if E_dec v v1 then reachableb_accum fuel' v1 v' else false) enum_vertices
-  end.
-
-Lemma reachableb_accum_elim (fuel : nat) (v : V) (v' : V)
-  (REACHABLE : reachableb_accum fuel v v' = true)
-  : exists w, L.length w <= fuel /\ v ~~~[ w ]~~>*( GRAPH ) v'.
-Proof.
-  exact (DigraphFixedpoint.reachableb_elim enum_vertices fuel v v' REACHABLE).
-Qed.
-
-Lemma reachableb_accum_intro (fuel : nat) (v : V) (v' : V) (w : list V)
-  (WALK : v ~~~[ w ]~~>*( GRAPH ) v')
-  (LENGTH : L.length w <= fuel)
-  : reachableb_accum fuel v v' = true.
-Proof.
-  exact (DigraphFixedpoint.reachableb_intro enum_vertices enum_vertices_has_edge_tgt fuel v v' w WALK LENGTH).
-Qed.
-
-Definition reachableb : forall v : V, forall v' : V, bool :=
-  reachableb_accum (L.length enum_vertices).
-
-Theorem reachableb_spec (v : V) (v' : V)
-  : reachableb v v' = true <-> v' \in reachable v.
-Proof.
-  exact (DigraphFixedpoint.reachableb_iff_reachable enum_vertices enum_vertices_has_edge_tgt v v').
-Qed.
-
-Definition reachable_impl (v : V) : fin_ensemble V :=
-  v :: L.filter (reachableb v) enum_vertices.
-
-Theorem reachable_sim
-  : forall v, reachable_impl v =~= reachable v.
-Proof.
-  exact (DigraphFixedpoint.reachable_sim enum_vertices enum_vertices_has_edge_tgt).
-Qed.
-
-Section DIGRAPH.
-
-#[local] Infix "\subseteq" := E.isSubsetOf.
-
-Context {A : Type}.
-
-Definition gmu_impl (seed_impl : V -> fin_ensemble A) (v : V) : fin_ensemble A :=
-  L.flat_map seed_impl (reachable_impl v).
-
-Variable seed : V -> ensemble A.
-
-Lemma walk_gmu (v : V) (v' : V) (w : list V)
-  (WALK : v ~~~[ w ]~~>*( GRAPH ) v')
-  : gmu seed v' \subseteq gmu seed v.
-Proof.
-  exact (DigraphFixedpoint.walk_gmu seed v v' w WALK).
-Qed.
-
-Lemma reachable_seed_gmu (v : V) (v' : V) (a : A)
-  (REACHABLE : v' \in reachable v)
-  (SEED : a \in seed v')
-  : a \in gmu seed v.
-Proof.
-  exact (DigraphFixedpoint.reachable_seed_gmu seed v v' a REACHABLE SEED).
-Qed.
-
-Lemma gmu_reachable_seed (v : V) (a : A)
-  (IN : a \in gmu seed v)
-  : exists v', v' \in reachable v /\ a \in seed v'.
-Proof.
-  exact (DigraphFixedpoint.gmu_reachable_seed seed v a IN).
-Qed.
-
-Lemma gmu_iff_reachable_seed (v : V) (a : A)
-  : a \in gmu seed v <-> a \in (reachable v >>= seed).
-Proof.
-  exact (DigraphFixedpoint.gmu_iff_reachable_seed seed v a).
-Qed.
-
-Theorem gmu_sim (seed_impl : V -> fin_ensemble A)
-  (seed_sim : forall v, seed_impl v =~= seed v)
-  : forall v, gmu_impl seed_impl v =~= gmu seed v.
-Proof.
-  exact (DigraphFixedpoint.gmu_sim seed seed_impl seed_sim enum_vertices enum_vertices_has_edge_tgt).
-Qed.
-
-#[local] Abbreviation is_fixedpoint value := (forall v, forall a, a \in value v <-> ⟪ STEP : a \in seed v \/ (exists v', (v, v') \in E /\ a \in value v') ⟫).
-
-Theorem gmu_is_fixedpoint
-  : is_fixedpoint (gmu seed).
-Proof.
-  exact (DigraphFixedpoint.gmu_is_fixedpoint seed).
-Qed.
-
-Theorem gmu_is_least_fixedpoint (value : V -> ensemble A)
-  (FIXPOINT : is_fixedpoint value)
-  : forall v, gmu seed v \subseteq value v.
-Proof.
-  exact (DigraphFixedpoint.gmu_is_least_fixedpoint seed value FIXPOINT).
-Qed.
-
-End DIGRAPH.
-
-Section DIGRAPH_FIXEDPOINT.
-
-#[local] Infix "∈" := L.In.
-#[local] Infix "\subseteq" := E.isSubsetOf.
-
-Definition deps (v : V) : fin_ensemble V :=
-  L.filter (fun v' => if E_dec v v' then true else false) enum_vertices.
-
-Lemma in_deps_iff (v : V) (v' : V)
-  : v' ∈ deps v <-> (v, v') \in E.
-Proof.
-  unfold deps. rewrite L.filter_In.
-  destruct (E_dec _ _) as [YES | NO]; ss!.
-  eapply enum_vertices_has_edge_tgt; eauto.
-Qed.
-
-#[local] Hint Rewrite in_deps_iff : simplication_hints.
-
-Context {A : Type}.
-
-Variable seed : V -> fin_ensemble A.
-
-Definition digraph_cl (v : V) : ensemble A :=
-  fun a => DigraphFixedpoint.digraph_closure seed deps a v.
-
-Definition digraph_trace (v : V) : A -> list V -> Prop :=
-  fun a => DigraphFixedpoint.digraph_trace seed deps a v.
-
-Theorem digraph_cl_iff_digraph_trace (v : V) (a : A)
-  : a \in digraph_cl v <-> (exists tr, tr \in digraph_trace v a).
-Proof.
-  exact (DigraphFixedpoint.digraph_closure_iff_trace seed deps v a).
-Qed.
-
-Lemma digraph_trace_seed_at_last (v : V) (a : A) (tr : list V)
-  (TRACE : tr \in digraph_trace v a)
-  : a ∈ seed (last tr v).
-Proof.
-  eapply DigraphFixedpoint.digraph_trace_seed_at_last; eauto.
-Qed.
-
-#[local] Hint Constructors walk : core.
-#[local] Hint Rewrite @L.last_cons : simplication_hints.
-
-Lemma digraph_trace_walk (v : V) (a : A) (tr : list V)
-  (TRACE : tr \in digraph_trace v a)
-  : v ~~~[ tr ]~~>*( GRAPH ) L.last tr v.
-Proof.
-  induction TRACE as [x IN | x y tr EDGE TRACE IH]; ss!.
-Qed.
-
-Lemma digraph_trace_simple (v : V) (a : A) (tr : list V)
-  (TRACE : tr \in digraph_trace v a)
-  : exists simple, simple \in digraph_trace v a /\ NoDup simple.
-Proof.
-  eapply DigraphFixedpoint.digraph_trace_simple; eauto.
-Qed.
-
-Lemma digraph_trace_in_nodes (nodes : fin_ensemble V) (v : V) (a : A) (tr : list V)
-  (deps_CLOSED : forall x, forall y, y ∈ deps x -> y ∈ nodes)
-  (TRACE : tr \in digraph_trace v a)
-  : Forall (fun y => y ∈ nodes) tr.
-Proof.
-  eapply DigraphFixedpoint.digraph_trace_in_nodes; eauto.
-Qed.
-
-Lemma digraph_trace_simple_bounded (nodes : fin_ensemble V) (v : V) (a : A) (tr : list V)
-  (deps_CLOSED : forall x, forall y, y ∈ deps x -> y ∈ nodes)
-  (TRACE : tr \in digraph_trace v a)
-  : exists simple, simple \in digraph_trace v a /\ length simple <= length nodes.
-Proof.
-  eapply DigraphFixedpoint.digraph_trace_simple_bounded; eauto.
-Qed.
-
-Definition is_digraph_fixedpoint (value : V -> ensemble A) : Prop :=
-  forall v, forall a, a \in value v <-> ⟪ STEP : a ∈ seed v \/ (exists v', v' ∈ deps v /\ a \in value v') ⟫.
-
-Theorem digraph_cl_is_fixedpoint
-  : is_digraph_fixedpoint digraph_cl.
-Proof.
-  exact (DigraphFixedpoint.digraph_closure_fixedpoint seed deps).
-Qed.
-
-Theorem digraph_cl_is_least_fixedpoint (value : V -> ensemble A)
-  (FIXPOINT : is_digraph_fixedpoint value)
-  : forall v, digraph_cl v \subseteq value v.
-Proof.
-  exact (DigraphFixedpoint.digraph_closure_least_fixedpoint seed deps value FIXPOINT).
-Qed.
-
-Variable A_dec : hasEqDec A.
-
-Definition digraph_cl_accum (fuel : nat) (v : V) : fin_ensemble A :=
-  DigraphFixedpoint.digraph_value fuel seed deps v.
-
-Lemma digraph_cl_accum_seed (fuel : nat) (v : V) (a : A)
-  (IN : a ∈ seed v)
-  : a ∈ digraph_cl_accum fuel v.
-Proof.
-  exact (DigraphFixedpoint.digraph_value_seed fuel seed deps v a IN).
-Qed.
-
-Lemma digraph_cl_accum_propagated (fuel : nat) (v : V) (v' : V) (a : A)
-  (EDGE : v' ∈ deps v)
-  (IN : a ∈ digraph_cl_accum fuel v')
-  : a ∈ digraph_cl_accum (S fuel) v.
-Proof.
-  exact (DigraphFixedpoint.digraph_value_propagated fuel seed deps v v' a EDGE IN).
-Qed.
-
-Theorem digraph_cl_accum_elim (fuel : nat) (v : V) (a : A)
-  (IN : a ∈ digraph_cl_accum fuel v)
-  : a \in digraph_cl v.
-Proof.
-  exact (DigraphFixedpoint.digraph_value_elim fuel seed deps v a IN).
-Qed.
-
-Lemma digraph_cl_accum_monotone (fuel : nat) (fuel' : nat) (v : V) (a : A)
-  (LE : fuel <= fuel')
-  (IN : a ∈ digraph_cl_accum fuel v)
-  : a ∈ digraph_cl_accum fuel' v.
-Proof.
-  exact (DigraphFixedpoint.digraph_value_monotone fuel fuel' seed deps v a LE IN).
-Qed.
-
-Lemma digraph_trace_diagraph_cl_accum (v : V) (a : A) (tr : list V) (fuel : nat)
-  (TRACE : tr \in digraph_trace v a)
-  (LE : length tr <= fuel)
-  : a ∈ digraph_cl_accum fuel v.
-Proof.
-  exact (DigraphFixedpoint.digraph_trace_value seed deps v a tr fuel TRACE LE).
-Qed.
-
-Theorem digraph_cl_intro (v : V) (a : A)
-  (IN : a \in digraph_cl v)
-  : exists fuel, a ∈ digraph_cl_accum fuel v.
-Proof.
-  exact (DigraphFixedpoint.digraph_closure_intro seed deps v a IN).
-Qed.
-
-Theorem digraph_cl_accum_good (fuel : nat) (nodes : fin_ensemble V) (v : V) (a : A)
-  (fuel_ENOUGH : length nodes <= fuel)
-  (deps_CLOSED : forall x, forall y, y ∈ deps x -> y ∈ nodes)
-  : a ∈ digraph_cl_accum fuel v <-> a \in digraph_cl v.
-Proof.
-  split.
-  - exact (digraph_cl_accum_elim fuel v a).
-  - exact (DigraphFixedpoint.digraph_closure_intro_bounded fuel nodes seed deps v a fuel_ENOUGH deps_CLOSED).
-Qed.
-
-Definition digraph_cl_impl : forall v : V, fin_ensemble A :=
-  digraph_cl_accum (length enum_vertices).
-
-Theorem digraph_cl_impl_spec (v : V) (a : A)
-  : a ∈ digraph_cl_impl v <-> a \in digraph_cl v.
-Proof.
-  eapply digraph_cl_accum_good with (nodes := enum_vertices).
-  - reflexivity.
-  - ii. rewrite in_deps_iff in H. eapply enum_vertices_has_edge_tgt. exact H.
-Qed.
-
-Corollary digraph_cl_sim
-  : forall v, digraph_cl_impl v =~= digraph_cl v.
-Proof.
-  i; s!. eapply digraph_cl_impl_spec with (v := v).
-Qed.
-
-End DIGRAPH_FIXEDPOINT.
-
-End EXPORT.
-
-End GraphAPI.
