theories/Data/FiniteSet.v
@@ -285,16 +285,4 @@ Proof.
   - ii; eapply INJ; ss!.
 Qed.
 
-Lemma subset_lemma (A : Type@{U_fs}) (xs : fin_ensemble A) (X : ensemble A)
-  : (exists X' : ensemble@{U_fs} A, xs =~= E.union X X') <-> (forall x : A, E.In x X -> L.In x xs).
-Proof.
-  ss!. exists (E.fromList xs). ss!.
-Qed.
-
-Lemma superset_lemma (A : Type@{U_fs}) (xs : fin_ensemble A) (X : ensemble A)
-  : (exists X' : ensemble@{U_fs} A, xs =~= E.intersection X X') <-> (forall x : A, L.In x xs -> E.In x X).
-Proof.
-  ss!. exists (E.fromList xs). ss!.
-Qed.
-
 End FS.
